LeanMqtt/Packets/Proofs.lean
@@ -4,13 +4,13 @@ import LeanMqtt.Packets.VarHeader.Proofs
 
 namespace Mqtt
 
-def Header.roundtrip (h : Header) (rest : List UInt8) :
+def Header.roundtrip (h : Header) {rest : List UInt8} :
     Header.parser.run (h.serialize ++ rest) = some (h, rest) := by
   simp [parser, serialize]
   simp [FixedHeader.roundtrip]
   simp [VarHeader.roundtrip]
 
-theorem Header.reconstruct (input : List UInt8) (h : Header) (rest : List UInt8) :
+theorem Header.reconstruct {h : Header} {input rest : List UInt8} :
     Header.parser.run input = some (h, rest) → input = h.serialize ++ rest := by
 
   simp only [parser, serialize]
@@ -24,8 +24,8 @@ theorem Header.reconstruct (input : List UInt8) (h : Header) (rest : List UInt8)
 
   cases h_eq
 
-  have h_fix_rec := FixedHeader.reconstruct _ _ _ h_fix
-  have h_var_rec := VarHeader.reconstruct _ _ _ _ h_var
+  have h_fix_rec := FixedHeader.reconstruct h_fix
+  have h_var_rec := VarHeader.reconstruct h_var
 
   rw [h_fix_rec, h_var_rec]
 
