LeanMqtt/Packets/VarHeader/Property/Proofs.lean
@@ -5,7 +5,7 @@ import LeanMqtt.Packets.VarHeader.Property.Basic
 namespace Mqtt
 open Mqtt
 
-def Property.roundtrip_kind (k : Kind) (val : Property.typeOfKind k) (rest : List UInt8) :
+def Property.roundtrip_kind {k : Kind} (val : Property.typeOfKind k) {rest : List UInt8} :
     (Property.parserKind k).run (Property.serializeKind k val ++ rest) = some (val, rest) := by
   simp [Property.parserKind, Property.serializeKind]
   split
@@ -19,28 +19,28 @@ def Property.roundtrip_kind (k : Kind) (val : Property.typeOfKind k) (rest : Lis
   · simp only [StrPair.roundtrip]
   · contradiction
 
-theorem Property.reconstruct_kind (k : Property.Kind) (input : List UInt8)
-    (val : Property.typeOfKind k) (rest : List UInt8) :
+theorem Property.reconstruct_kind {k : Property.Kind}
+    {val : Property.typeOfKind k} {input rest : List UInt8} :
     (Property.parserKind k).run input = some (val, rest) →
     input = Property.serializeKind k val ++ rest := by
   cases k <;> simp only [Property.parserKind, Property.serializeKind]
-  · exact UInt8.reconstruct input val rest
-  · exact UInt16.reconstruct input val rest
-  · exact UInt32.reconstruct input val rest
-  · exact VarInt.reconstruct input val rest
-  · exact BinaryData.reconstruct input val rest
-  · exact Str.reconstruct input val rest
-  · exact StrPair.reconstruct input val rest
+  · exact UInt8.reconstruct
+  · exact UInt16.reconstruct
+  · exact UInt32.reconstruct
+  · exact VarInt.reconstruct
+  · exact BinaryData.reconstruct
+  · exact Str.reconstruct
+  · exact StrPair.reconstruct
   · intro h; contradiction
 
-theorem Property.roundtrip (p : Property) (rest : List UInt8) :
+theorem Property.roundtrip (p : Property) {rest : List UInt8} :
     Property.parser.run (p.serialize ++ rest) = some (p, rest) := by
   simp [Property.parser, Property.serialize]
   simp [Option.bind, Option.map]
   simp [VarInt.roundtrip]
   simp [Property.roundtrip_kind]
 
-theorem Property.reconstruct (input : List UInt8) (p : Property) (rest : List UInt8) :
+theorem Property.reconstruct {p : Property} {input rest : List UInt8} :
     Property.parser.run input = some (p, rest) → input = p.serialize ++ rest := by
 
   simp only [Property.parser, Property.serialize]
@@ -51,16 +51,16 @@ theorem Property.reconstruct (input : List UInt8) (p : Property) (rest : List UI
   obtain ⟨h_p, h_rest⟩ := Parser.pure_run_success h_next2
 
   subst h_rest
-  have h_rec_id := VarInt.reconstruct _ _ _ h_id
-  have h_rec_val := Property.reconstruct_kind (getKind id) _ _ _ h_val
+  have h_rec_id := VarInt.reconstruct h_id
+  have h_rec_val := Property.reconstruct_kind h_val
 
   rw [h_rec_id, h_rec_val, h_p]
   simp [List.append_assoc]
 
-theorem Property.parser_len_consumed (input : List UInt8) (p : Property) (rest : List UInt8) :
+theorem Property.parser_len_consumed {p : Property} {input rest : List UInt8} :
     Property.parser.run input = some (p, rest) → input.length = p.byteSize + rest.length := by
   intro h
-  have h_eq := Property.reconstruct _ _ _ h
+  have h_eq := Property.reconstruct h
   simp [h_eq, List.length_append]
 
 theorem Property.byteSize_pos (p : Property) : 0 < p.byteSize := by
@@ -70,10 +70,12 @@ theorem Property.byteSize_pos (p : Property) : 0 < p.byteSize := by
   unfold VarInt.serialize
   grind
 
-instance : ChunkItem Property where
+instance : Codec Property where
   parser      := Property.parser
   serialize   := Property.serialize
-  h_pos       := Property.byteSize_pos
-  h_consumed  := Property.parser_len_consumed
   roundtrip   := Property.roundtrip
   reconstruct := Property.reconstruct
+
+instance : ChunkItem Property where
+  h_pos      := Property.byteSize_pos
+  h_consumed := Property.parser_len_consumed
