LeanMqtt/Primitives/Proofs.lean
@@ -14,11 +14,11 @@ theorem UInt8.parser_len (n : UInt8) :
     n.serialize.length = 1 := by
   rfl
 
-theorem UInt8.roundtrip (b : UInt8) (rest : List UInt8) :
+theorem UInt8.roundtrip (b : UInt8) {rest : List UInt8} :
     UInt8.parser.run (b.serialize ++ rest) = some (b, rest) := by
     simp [UInt8.parser, UInt8.serialize]
 
-theorem UInt8.reconstruct (input : List UInt8) (b : UInt8) (rest : List UInt8) :
+theorem UInt8.reconstruct {b : UInt8} {input rest : List UInt8} :
     UInt8.parser.run input = some (b, rest) → input = b.serialize ++ rest := by
   simp [UInt8.parser, UInt8.serialize, StateT.run_bind, StateT.run_get]
   split
@@ -34,7 +34,7 @@ theorem UInt16.parser_len (n : UInt16) :
     n.serialize.length = 2 := by
   rfl
 
-theorem UInt16.roundtrip (n : UInt16) (rest : List UInt8) :
+theorem UInt16.roundtrip (n : UInt16) {rest : List UInt8} :
     UInt16.parser.run (n.serialize ++ rest) = some (n, rest) := by
   simp [UInt16.parser]
   rw [←UInt16.parser_len n]
@@ -42,7 +42,7 @@ theorem UInt16.roundtrip (n : UInt16) (rest : List UInt8) :
   simp [UInt16.serialize]
   bv_decide
 
-theorem UInt16.reconstruct (input : List UInt8) (n : UInt16) (rest : List UInt8) :
+theorem UInt16.reconstruct {n : UInt16} {input rest : List UInt8} :
     UInt16.parser.run input = some (n, rest) → input = n.serialize ++ rest := by
 
   simp only [UInt16.parser, UInt16.serialize]
@@ -67,7 +67,7 @@ theorem UInt32.parser_len (n : UInt32) :
     n.serialize.length = 4 := by
   rfl
 
-theorem UInt32.roundtrip (n : UInt32) (rest : List UInt8) :
+theorem UInt32.roundtrip (n : UInt32) {rest : List UInt8} :
     UInt32.parser.run (n.serialize ++ rest) = some (n, rest) := by
   simp [UInt32.parser]
   rw [←UInt32.parser_len n]
@@ -75,7 +75,7 @@ theorem UInt32.roundtrip (n : UInt32) (rest : List UInt8) :
   simp [UInt32.serialize]
   bv_decide
 
-theorem UInt32.reconstruct (input : List UInt8) (n : UInt32) (rest : List UInt8) :
+theorem UInt32.reconstruct {n : UInt32} {input rest : List UInt8} :
     UInt32.parser.run input = some (n, rest) → input = n.serialize ++ rest := by
 
   simp only [UInt32.parser, UInt32.serialize]
@@ -103,7 +103,7 @@ theorem String.serialize_len (s : String) :
   unfold String.utf8ByteSize
   exact @Array.size_eq_length_toList UInt8 s.toByteArray.data
 
-theorem String.parser_len (len : Nat) (s : String) (inp rest : List UInt8) :
+theorem String.parser_len {len : Nat} {s : String} {inp rest : List UInt8} :
     (String.parser len).run inp = some (s, rest) → s.utf8ByteSize = len := by
   simp [String.parser]
   simp [Option.bind]
@@ -121,7 +121,7 @@ theorem String.parser_len (len : Nat) (s : String) (inp rest : List UInt8) :
       exact h_len
     · contradiction
 
-theorem String.roundtrip (s : String) (rest : List UInt8) :
+theorem String.roundtrip (s : String) {rest : List UInt8} :
     (String.parser s.serialize.length).run (s.serialize ++ rest) = some (s, rest) := by
   simp only [String.serialize, String.parser]
   simp [String.toUTF8_eq_toByteArray, Option.bind]
@@ -134,7 +134,7 @@ theorem String.roundtrip (s : String) (rest : List UInt8) :
     simp [Helpers.bytearray_list_roundtrip] at h
     exact absurd s.isValidUTF8 h
 
-theorem String.roundtrip_proof (s : String) (rest : List UInt8) :
+theorem String.roundtrip_proof (s : String) {rest : List UInt8} :
     (String.parserWithProof s.serialize.length).run (s.serialize ++ rest) =
     some (⟨s, s.serialize_len.symm⟩, rest) := by
   simp [String.parserWithProof]
@@ -159,8 +159,8 @@ theorem String.roundtrip_proof (s : String) (rest : List UInt8) :
       simp [String.serialize, Helpers.bytearray_list_roundtrip] at h_wrong
       exact absurd s.isValidUTF8 h_wrong
 
-theorem String.reconstructWithProof (len : Nat) (input : List UInt8)
-    (s : { s : String // s.utf8ByteSize = len }) (rest : List UInt8) :
+theorem String.reconstructWithProof {len : Nat} {s : { s : String // s.utf8ByteSize = len }}
+    {input rest : List UInt8} :
     (String.parserWithProof len).run input = some (s, rest) → input = s.val.serialize ++ rest := by
 
   simp only [String.parserWithProof, String.serialize]
@@ -178,12 +178,12 @@ theorem String.reconstructWithProof (len : Nat) (input : List UInt8)
     simp [String.fromUTF8, String.toUTF8_eq_toByteArray, Helpers.list_bytearray_roundtrip]
   · contradiction
 
-theorem String.parserWithProof_eq_parser_success (n : Nat) (inp : List UInt8)
-    (s : String) (rest : List UInt8) :
+theorem String.parserWithProof_eq_parser_success {n : Nat} {s : String}
+    {inp rest : List UInt8} :
     (String.parser n).run inp = some (s, rest) →
     ∃ h, (String.parserWithProof n).run inp = some (⟨s, h⟩, rest) := by
   intro h_simple
-  have h_parser_len := String.parser_len _ _ _ _ h_simple
+  have h_parser_len := String.parser_len h_simple
 
   -- Unfold both parsers
   simp only [String.parser, String.parserWithProof] at *
@@ -216,7 +216,7 @@ theorem Str.roundtrip (s : Str) (rest : List UInt8) :
     Option.map_eq_map, Option.bind_eq_bind
   ]
 
-  rw [UInt16.roundtrip _ _]
+  rw [UInt16.roundtrip s.len.val]
   simp only [Option.bind_some, Option.map]
 
   have h_len_eq : s.len.val.toNat = s.val.serialize.length := by
@@ -233,14 +233,14 @@ theorem Str.roundtrip (s : Str) (rest : List UInt8) :
     lemma (`String.parserWithProof_eq_parser_success`) to show it also holds for
     `String.parserWithProof`.
   -/
-  have h_simple := String.roundtrip s.val rest
+  have h_simple := @String.roundtrip s.val rest
 
   rw [←h_len_eq] at h_simple
-  have ⟨_, h_dep⟩ := String.parserWithProof_eq_parser_success _ _ _ _ h_simple
+  have ⟨_, h_dep⟩ := String.parserWithProof_eq_parser_success h_simple
 
   rw [h_dep]
 
-theorem Str.reconstruct (input : List UInt8) (s : Str) (rest : List UInt8) :
+theorem Str.reconstruct {s : Str} {input rest : List UInt8} :
     Str.parser.run input = some (s, rest) → input = s.serialize ++ rest := by
 
   simp only [Str.parser, Str.serialize]
@@ -251,18 +251,18 @@ theorem Str.reconstruct (input : List UInt8) (s : Str) (rest : List UInt8) :
   obtain ⟨h_s, h_rest⟩ := Parser.pure_run_success h_next2
 
   subst h_rest
-  have h_rec_len := UInt16.reconstruct _ _ _ h_len
-  have h_rec_str := String.reconstructWithProof _ _ _ _ h_str
+  have h_rec_len := UInt16.reconstruct h_len
+  have h_rec_str := String.reconstructWithProof h_str
 
   rw [h_rec_len, h_rec_str, h_s]
   simp [List.append_assoc]
 
-theorem StrPair.roundtrip (p : StrPair) (rest : List UInt8) :
+theorem StrPair.roundtrip (p : StrPair) {rest : List UInt8} :
     StrPair.parser.run (p.serialize ++ rest) = some (p, rest) := by
   simp [StrPair.parser, StrPair.serialize, Option.bind, Option.map]
   simp only [Str.roundtrip _ _]
 
-theorem StrPair.reconstruct (input : List UInt8) (p : StrPair) (rest : List UInt8) :
+theorem StrPair.reconstruct {p : StrPair} {input rest : List UInt8} :
     StrPair.parser.run input = some (p, rest) → input = p.serialize ++ rest := by
   simp only [StrPair.parser, StrPair.serialize]
   intro h
@@ -273,17 +273,17 @@ theorem StrPair.reconstruct (input : List UInt8) (p : StrPair) (rest : List UInt
   obtain ⟨h_p, h_rest⟩ := Parser.pure_run_success h_next2
   subst h_p h_rest
 
-  have rec1 := Str.reconstruct input s1 mid1 h_s1
-  have rec2 := Str.reconstruct mid1 s2 mid2 h_s2
+  have rec1 := Str.reconstruct h_s1
+  have rec2 := Str.reconstruct h_s2
 
   rw [rec1, rec2, List.append_assoc]
 
-theorem BinaryData.roundtrip (b : BinaryData) (rest : List UInt8) :
+theorem BinaryData.roundtrip (b : BinaryData) {rest : List UInt8} :
     BinaryData.parser.run (b.serialize ++ rest) = some (b, rest) := by
   simp only [BinaryData.parser, BinaryData.serialize]
   simp [Option.bind, Option.map]
 
-  rw [UInt16.roundtrip _ _]
+  rw [UInt16.roundtrip]
   simp only
 
   have h_len_eq : b.len.val.toNat = b.val.toList.length := by
@@ -302,7 +302,7 @@ theorem BinaryData.roundtrip (b : BinaryData) (rest : List UInt8) :
 
   rw [h_dep]
 
-theorem BinaryData.reconstruct (input : List UInt8) (b : BinaryData) (rest : List UInt8) :
+theorem BinaryData.reconstruct {b : BinaryData} {input rest : List UInt8} :
     BinaryData.parser.run input = some (b, rest) → input = b.serialize ++ rest := by
 
   simp only [BinaryData.parser, BinaryData.serialize]
@@ -313,13 +313,13 @@ theorem BinaryData.reconstruct (input : List UInt8) (b : BinaryData) (rest : Lis
   obtain ⟨h_b, h_rest⟩ := Parser.pure_run_success h_next2
 
   subst h_rest
-  have h_rec_len := UInt16.reconstruct _ _ _ h_len
+  have h_rec_len := UInt16.reconstruct h_len
   have h_rec_bytes := Parser.bytesWithProof_reconstruct h_bytes
 
   rw [h_rec_len, h_rec_bytes, h_b]
   simp [List.append_assoc]
 
-theorem VarInt.roundtrip (v : VarInt) (rest : List UInt8) :
+theorem VarInt.roundtrip (v : VarInt) {rest : List UInt8} :
     VarInt.parser.run (v.serialize ++ rest) = some (v, rest) := by
 
   have ⟨v', h_v_limit⟩ := v
@@ -429,8 +429,7 @@ theorem VarInt.roundtrip (v : VarInt) (rest : List UInt8) :
           -- Since `v` is limited by `VarInt.limit`, h₄ must be false.
           grind
 
-theorem VarInt.reconstruct
-    (input : List UInt8) (v : VarInt) (rest : List UInt8) :
+theorem VarInt.reconstruct {v : VarInt} {input rest : List UInt8} :
     VarInt.parser.run input = some (v, rest) → input = v.serialize ++ rest := by
 
   intro h_parse
